theories/exercises/subseg_buffer_IE_closure.v
@@ -1,0 +1,74 @@
+From iris.algebra Require Import frac.
+From iris.proofmode Require Import tactics.
+Require Import Eqdep_dec List.
+From cap_machine Require Import register_tactics.
+From cap_machine Require Import fundamental logrel rules.
+From cap_machine.proofmode Require Import tactics_helpers proofmode.
+From cap_machine.examples Require Import template_adequacy.
+From cap_machine.exercises Require Import subseg_buffer.
+Open Scope Z_scope.
+
+(** Firtly, we create a closure around our code and buffer. The capability
+    pointing to the allocated buffer is stored in memory. We thus have to load
+    it in the register. This part of code sets up the context, allowing to use
+    the previous specification.
+ *)
+Section closure_program.
+
+  Context {Σ:gFunctors} {memg:memG Σ} {regg:regG Σ} {sealsg: sealStoreG Σ}
+          `{MP: MachineParameters}.
+  Context {nainv: logrel_na_invs Σ}.
+
+  Program Definition inv_ie_pc b_pc e_pc a_pc
+    : leibnizO Word -n> iPropO Σ :=
+    λne w, ⌜w = (WCap RX b_pc e_pc a_pc)⌝%I.
+
+  Program Definition inv_ie_idc b_mem e_mem
+    : leibnizO Word -n> iPropO Σ :=
+    λne w, ⌜w = (WCap RW b_mem e_mem b_mem)⌝%I.
+
+  Lemma prog_CPS_safe_to_share_IE
+    b_pc e_pc a_prog (b_mem e_mem: Addr) secret_off secret
+    b_ie e_ie a_ie :
+
+    (* The instructions of the code are in the memory closure of the PCC *)
+    SubBounds b_pc e_pc a_prog (a_prog ^+ length (prog_code secret_off secret))% a →
+    (* The secret offset fits in the memory buffer *)
+    (b_mem ≤ b_mem ^+ secret_off < e_mem)%a →
+
+    SubBounds b_ie e_ie a_ie (a_ie ^+ 1)%a →
+
+    ⊢ ( code_inv a_prog secret_off secret
+       ∗ start_mem_inv b_mem e_mem secret_off
+       ∗ end_mem_inv b_mem e_mem secret_off
+       ∗ secret_inv b_mem secret_off secret
+       ∗ inv (logN.@a_ie) (∃ w1 : leibnizO Word , a_ie ↦ₐ w1 ∗ inv_ie_pc b_pc e_pc a_prog w1)
+       ∗ inv (logN.@(a_ie ^+ 1)%a) (∃ w2 : leibnizO Word, (a_ie ^+ 1)%a ↦ₐ w2 ∗ inv_ie_idc b_mem e_mem w2)
+      )
+
+   -∗ interp (WCap IE b_ie e_ie a_ie).
+  Proof.
+    iIntros (Hbounds_pc Hbounds_mem Hbounds_ie)
+      "#(Hcode & Hmem & Hend_mem & Hsecret & Hinv_ie_pc & Hinv_ie_idc)".
+    rewrite fixpoint_interp1_eq /=.
+    iIntros "[%Hwb %Hwb']".
+    iExists (inv_ie_pc b_pc e_pc a_prog), (inv_ie_idc b_mem e_mem).
+    iSplit.
+    rewrite /persistent_cond /inv_ie_pc //=.
+    iPureIntro; intros; apply bi.pure_persistent.
+    iSplit.
+    rewrite /persistent_cond /inv_ie_pc //=.
+    iPureIntro; intros; apply bi.pure_persistent.
+    iFrame "#".
+    iIntros (w1 w2 regs). iNext ; iModIntro.
+    iIntros "[Hw1 Hw2] ([Hfull Hregs] & Hrmap & Hown)".
+    rewrite /=.
+
+    (* TODO And the problem arise at this point, if I have the disjunction:
+       (P1 w1 \/ interp w1) * (P2 w2 \/ interp w2) -* E(w1, w2)
+       I need the cases [w1 = ...] and [w2 = ... ],
+       otherwise, the spec says nothing.
+     *)
+
+    iApply (prog_spec_CPS_full with "[-]") ; eauto.
+End closure_program.
